\section{Sequences, Induction and Recursion}
\begin{itemize}
\bulletitem Sequences
\begin{itemize}
\bulletitem Definition \( D:f(x) \)
\bulletitem Properties
\end{itemize}
\bulletitem Summations \( \sum \)
\bulletitem Telescopic sums \( \sum_{k=1}^{n} \frac{1}{k(k+1)} = \frac{1}{1}-\frac{1}{n+1} \)
\bulletitem Product \( \prod \)
\bulletitem Theorems
\begin{itemize}
\bulletitem Adding and removing a final term
\bulletitem \( \sum_{k=m}^{n} a_k + \sum_{k=m}^{n} b_k = \sum_{k=m}^{n} a_k + b_k \)
\bulletitem \( c \dot \sum_{k=m}^{n} a_k = \sum_{k=m}^{n} c \dot a_k \)
\bulletitem \( \prod_{k=m}^{n} a_k + \prod_{k=m}^{n} b_k = \prod_{k=m}^{n} a_k + b_k \)
\end{itemize}
\bulletitem Factorials \( n! \)
\bulletitem Combinations \comb{n}{r}
\bulletitem Induction
\begin{itemize}
\bulletitem \( a,k \in \Z \)
\bulletitem If \( P(a) \)
\bulletitem and \( \forall k \geq a, P(k) \rightarrow P(k+1) \)
\bulletitem then \( \forall n \geq a, P(n) \)
\end{itemize}
\bulletitem Prove sum of first n integers by induction
\bulletitem Recursion
\end{itemize}